_:A16aa612cX3aX1625a2637d3X3aXX2dX7ff9 <http://www.w3.org/1999/02/22-rdf-syntax-ns#rest> <http://www.w3.org/1999/02/22-rdf-syntax-ns#nil> .
_:A16aa612cX3aX1625a2637d3X3aXX2dX7ff9 <http://www.w3.org/1999/02/22-rdf-syntax-ns#first> <http://w3id.org/abdn/policy/pope#XOR_Node> .
<http://w3id.org/abdn/policy/pope#WordFrequencyDataSet> <http://www.w3.org/2000/01/rdf-schema#label> "Word Frequency Dataset"@en .
<http://w3id.org/abdn/policy/pope#WordFrequencyDataSet> <http://www.w3.org/2000/01/rdf-schema#comment> "A kind of role describing that the associated prov:Entity denoted a prov:Collection representing  word frequency  results collection."@en .
<http://w3id.org/abdn/policy/pope#WordFrequencyDataSet> <http://www.w3.org/1999/02/22-rdf-syntax-ns#type> <http://w3id.org/abdn/policy/pope#DataSet> .
<http://w3id.org/abdn/policy/pope#WordFrequencyDataSet> <http://www.w3.org/1999/02/22-rdf-syntax-ns#type> <http://www.w3.org/2002/07/owl#NamedIndividual> .
<http://w3id.org/abdn/policy/pope#LeafNode> <http://www.w3.org/2000/01/rdf-schema#label> "Leaf Node"@en .
<http://w3id.org/abdn/policy/pope#LeafNode> <http://www.w3.org/2000/01/rdf-schema#comment> "A concept describing a leaf node of a binary tree structure. The node is used to bind a \na binary tree description of pope:Constraint to a specific pope:Parameter wich captures an aspect of the state of the world via subproperties of skos:related defined in PoPE. For eample, a parameter representing a keyword being included in a piece of text."@en .
<http://w3id.org/abdn/policy/pope#LeafNode> <http://www.w3.org/2002/07/owl#disjointWith> <http://w3id.org/abdn/policy/pope#XOR_Node> .
<http://w3id.org/abdn/policy/pope#LeafNode> <http://www.w3.org/2002/07/owl#disjointWith> <http://w3id.org/abdn/policy/pope#OR_Node> .
<http://w3id.org/abdn/policy/pope#LeafNode> <http://www.w3.org/2000/01/rdf-schema#subClassOf> <http://www.w3.org/2004/02/skos/core#Concept> .
<http://w3id.org/abdn/policy/pope#LeafNode> <http://www.w3.org/1999/02/22-rdf-syntax-ns#type> <http://www.w3.org/2002/07/owl#Class> .
_:A16aa612cX3aX1625a2637d3X3aXX2dX7ff3 <http://www.w3.org/2002/07/owl#unionOf> _:A16aa612cX3aX1625a2637d3X3aXX2dX7ff2 .
_:A16aa612cX3aX1625a2637d3X3aXX2dX7ff3 <http://www.w3.org/1999/02/22-rdf-syntax-ns#type> <http://www.w3.org/2002/07/owl#Class> .
_:A16aa612cX3aX1625a2637d3X3aXX2dX7fec <http://www.w3.org/1999/02/22-rdf-syntax-ns#rest> _:A16aa612cX3aX1625a2637d3X3aXX2dX7feb .
_:A16aa612cX3aX1625a2637d3X3aXX2dX7fec <http://www.w3.org/1999/02/22-rdf-syntax-ns#first> <http://w3id.org/abdn/policy/pope#OR_Node> .
<http://w3id.org/abdn/policy/pope#doesNotMatch> <http://www.w3.org/2000/01/rdf-schema#label> "doesNotMatch"@en .
<http://w3id.org/abdn/policy/pope#doesNotMatch> <http://www.w3.org/2000/01/rdf-schema#comment> "A matches B denotes that the expression described by the instance A cannot be matched on some value described by the instance B. For example, if A describes a regular expression, it cannnot be matched on a piece of text described by B."@en .
<http://w3id.org/abdn/policy/pope#doesNotMatch> <http://www.w3.org/2000/01/rdf-schema#subPropertyOf> <http://www.w3.org/2004/02/skos/core#related> .
<http://w3id.org/abdn/policy/pope#doesNotMatch> <http://www.w3.org/1999/02/22-rdf-syntax-ns#type> <http://www.w3.org/2002/07/owl#ObjectProperty> .
<http://w3id.org/abdn/policy/pope#rhs> <http://www.w3.org/2000/01/rdf-schema#label> "rhs"@en .
<http://w3id.org/abdn/policy/pope#rhs> <http://www.w3.org/2000/01/rdf-schema#comment> "A property linking a parent node of a binary tree to its right hand side child."@en .
<http://w3id.org/abdn/policy/pope#rhs> <http://www.w3.org/2000/01/rdf-schema#range> _:A16aa612cX3aX1625a2637d3X3aXX2dX7fef .
<http://w3id.org/abdn/policy/pope#rhs> <http://www.w3.org/2000/01/rdf-schema#domain> _:A16aa612cX3aX1625a2637d3X3aXX2dX7ff3 .
<http://w3id.org/abdn/policy/pope#rhs> <http://www.w3.org/1999/02/22-rdf-syntax-ns#type> <http://www.w3.org/2002/07/owl#FunctionalProperty> .
<http://w3id.org/abdn/policy/pope#rhs> <http://www.w3.org/2000/01/rdf-schema#subPropertyOf> <http://www.w3.org/2004/02/skos/core#related> .
<http://w3id.org/abdn/policy/pope#rhs> <http://www.w3.org/1999/02/22-rdf-syntax-ns#type> <http://www.w3.org/2002/07/owl#ObjectProperty> .
<http://w3id.org/abdn/policy/pope#TextObject> <http://www.w3.org/2000/01/rdf-schema#label> "Text Object"@en .
<http://w3id.org/abdn/policy/pope#TextObject> <http://www.w3.org/2000/01/rdf-schema#comment> "A role describing that the associated prov:Entity denoted an activity parameter containing some information about a piece of text used in some data processing activity."@en .
<http://w3id.org/abdn/policy/pope#TextObject> <http://www.w3.org/1999/02/22-rdf-syntax-ns#type> <http://w3id.org/abdn/policy/pope#Parameter> .
<http://w3id.org/abdn/policy/pope#TextObject> <http://www.w3.org/1999/02/22-rdf-syntax-ns#type> <http://www.w3.org/2002/07/owl#NamedIndividual> .
<http://w3id.org/abdn/policy/pope#SentimentAnalysis> <http://www.w3.org/2000/01/rdf-schema#label> "Sentiment Analysis"@en .
<http://w3id.org/abdn/policy/pope#SentimentAnalysis> <http://www.w3.org/2000/01/rdf-schema#comment> "A kind of activity plan describing analysis that utilises an algorithm to determine the sentiment (e.g. positive, negative, neutral) in a corpus of documents."@en .
<http://w3id.org/abdn/policy/pope#SentimentAnalysis> <http://www.w3.org/2000/01/rdf-schema#subClassOf> <http://w3id.org/abdn/policy/pope#DataAnalysis> .
<http://w3id.org/abdn/policy/pope#SentimentAnalysis> <http://www.w3.org/1999/02/22-rdf-syntax-ns#type> <http://www.w3.org/2002/07/owl#Class> .
<http://w3id.org/abdn/policy/pope#DataSet> <http://www.w3.org/2000/01/rdf-schema#label> "Data Set"@en .
<http://w3id.org/abdn/policy/pope#DataSet> <http://www.w3.org/2000/01/rdf-schema#comment> "A kind of role describing that the associated prov:Entity denoted a prov:Collection representing some dataset - i.e. a collection of dataset items."@en .
<http://w3id.org/abdn/policy/pope#DataSet> <http://www.w3.org/2000/01/rdf-schema#subClassOf> <http://www.w3.org/ns/prov#Role> .
<http://w3id.org/abdn/policy/pope#DataSet> <http://www.w3.org/1999/02/22-rdf-syntax-ns#type> <http://www.w3.org/2002/07/owl#Class> .
_:A16aa612cX3aX1625a2637d3X3aXX2dX7fe5 <http://www.w3.org/2000/01/rdf-schema#label> "Text to uppercase"@en .
_:A16aa612cX3aX1625a2637d3X3aXX2dX7fe5 <http://www.w3.org/2000/01/rdf-schema#comment> "A kind of activity plan describing a process converting text to uppercase. This kind of action is further described by prov:Entities used by the activity and described using pope:Parameter role, and associated PoPE subproperties of skos:related such as pope:includedIn, pope:subsumes, etc.   For example, and entity with role pope:Regex representing lowercase letters linked to some characteristics of entities (data items) generated by the activity via pope:doesNotMatch denotes that the generated entities contain a text that does not contain any lowercase letters (subject to further constriants imposed on the parameters described using pope:Constraint)."@en .
_:A16aa612cX3aX1625a2637d3X3aXX2dX7fe5 <http://www.w3.org/2002/07/owl#annotatedTarget> <http://w3id.org/abdn/policy/pope#DataPreprocessing> .
_:A16aa612cX3aX1625a2637d3X3aXX2dX7fe5 <http://www.w3.org/2002/07/owl#annotatedProperty> <http://www.w3.org/1999/02/22-rdf-syntax-ns#type> .
_:A16aa612cX3aX1625a2637d3X3aXX2dX7fe5 <http://www.w3.org/2002/07/owl#annotatedSource> <http://w3id.org/abdn/policy/pope#TextToUpperCase> .
_:A16aa612cX3aX1625a2637d3X3aXX2dX7fe5 <http://www.w3.org/1999/02/22-rdf-syntax-ns#type> <http://www.w3.org/2002/07/owl#Axiom> .
_:A16aa612cX3aX1625a2637d3X3aXX2dX7ff8 <http://www.w3.org/2002/07/owl#unionOf> _:A16aa612cX3aX1625a2637d3X3aXX2dX7ff7 .
_:A16aa612cX3aX1625a2637d3X3aXX2dX7ff8 <http://www.w3.org/1999/02/22-rdf-syntax-ns#type> <http://www.w3.org/2002/07/owl#Class> .
<http://w3id.org/abdn/policy/pope#appliesTo> <http://www.w3.org/2000/01/rdf-schema#label> "appliesTo"@en .
<http://w3id.org/abdn/policy/pope#appliesTo> <http://www.w3.org/2000/01/rdf-schema#comment> "A appliesTo B denotes that the instance A describes some concept relevant to B and where A is not part of B. For example, a license applied to a collection of data items."@en .
<http://w3id.org/abdn/policy/pope#appliesTo> <http://www.w3.org/2000/01/rdf-schema#subPropertyOf> <http://www.w3.org/2004/02/skos/core#related> .
<http://w3id.org/abdn/policy/pope#appliesTo> <http://www.w3.org/1999/02/22-rdf-syntax-ns#type> <http://www.w3.org/2002/07/owl#ObjectProperty> .
<http://w3id.org/abdn/policy/pope#DataCollection> <http://www.w3.org/2000/01/rdf-schema#label> "Data Collection"@en .
<http://w3id.org/abdn/policy/pope#DataCollection> <http://www.w3.org/2000/01/rdf-schema#comment> "A kind of  activity plan describing the process of data gathering (e.g. manual collection, collection using an API etc.)"@en .
<http://w3id.org/abdn/policy/pope#DataCollection> <http://www.w3.org/2000/01/rdf-schema#subClassOf> <http://w3id.org/abdn/policy/pope#ActivityPlan> .
<http://w3id.org/abdn/policy/pope#DataCollection> <http://www.w3.org/1999/02/22-rdf-syntax-ns#type> <http://www.w3.org/2002/07/owl#Class> .
<http://w3id.org/abdn/policy/pope#Parameter> <http://www.w3.org/2000/01/rdf-schema#label> "Parameter"@en .
<http://w3id.org/abdn/policy/pope#Parameter> <http://www.w3.org/2000/01/rdf-schema#comment> "A kind of role describing that the associated prov:Entity denoted an activity parameter containing some information used in some data processing activity."@en .
<http://w3id.org/abdn/policy/pope#Parameter> <http://www.w3.org/2000/01/rdf-schema#subClassOf> <http://www.w3.org/ns/prov#Role> .
<http://w3id.org/abdn/policy/pope#Parameter> <http://www.w3.org/1999/02/22-rdf-syntax-ns#type> <http://www.w3.org/2002/07/owl#Class> .
<http://w3id.org/abdn/policy/pope#NaiveBayesSentimentAnalysis> <http://www.w3.org/2000/01/rdf-schema#label> "Na\u00EFve Bayes Sentiment Analysis"@en .
<http://w3id.org/abdn/policy/pope#NaiveBayesSentimentAnalysis> <http://www.w3.org/2000/01/rdf-schema#comment> "A sentiment analysis utilising the na\u00EFve Bayes algorithm."@en .
<http://w3id.org/abdn/policy/pope#NaiveBayesSentimentAnalysis> <http://www.w3.org/1999/02/22-rdf-syntax-ns#type> <http://w3id.org/abdn/policy/pope#SentimentAnalysis> .
<http://w3id.org/abdn/policy/pope#NaiveBayesSentimentAnalysis> <http://www.w3.org/1999/02/22-rdf-syntax-ns#type> <http://w3id.org/abdn/policy/pope#DataAnalysis> .
<http://w3id.org/abdn/policy/pope#NaiveBayesSentimentAnalysis> <http://www.w3.org/1999/02/22-rdf-syntax-ns#type> <http://w3id.org/abdn/policy/pope#ActivityPlan> .
<http://w3id.org/abdn/policy/pope#NaiveBayesSentimentAnalysis> <http://www.w3.org/1999/02/22-rdf-syntax-ns#type> <http://www.w3.org/2002/07/owl#NamedIndividual> .
<http://w3id.org/abdn/policy/pope#NewsArticleDataSet> <http://www.w3.org/2000/01/rdf-schema#label> "News Article Dataset"@en .
<http://w3id.org/abdn/policy/pope#NewsArticleDataSet> <http://www.w3.org/2000/01/rdf-schema#comment> "A kind of role describing that the associated prov:Entity denoted a prov:Collection representing a collection of news articles."@en .
<http://w3id.org/abdn/policy/pope#NewsArticleDataSet> <http://www.w3.org/1999/02/22-rdf-syntax-ns#type> <http://w3id.org/abdn/policy/pope#DataSet> .
<http://w3id.org/abdn/policy/pope#NewsArticleDataSet> <http://www.w3.org/1999/02/22-rdf-syntax-ns#type> <http://www.w3.org/2002/07/owl#NamedIndividual> .
_:A16aa612cX3aX1625a2637d3X3aXX2dX7ff2 <http://www.w3.org/1999/02/22-rdf-syntax-ns#rest> _:A16aa612cX3aX1625a2637d3X3aXX2dX7ff1 .
_:A16aa612cX3aX1625a2637d3X3aXX2dX7ff2 <http://www.w3.org/1999/02/22-rdf-syntax-ns#first> <http://w3id.org/abdn/policy/pope#AND_Node> .
_:A16aa612cX3aX1625a2637d3X3aXX2dX7feb <http://www.w3.org/1999/02/22-rdf-syntax-ns#rest> <http://www.w3.org/1999/02/22-rdf-syntax-ns#nil> .
_:A16aa612cX3aX1625a2637d3X3aXX2dX7feb <http://www.w3.org/1999/02/22-rdf-syntax-ns#first> <http://w3id.org/abdn/policy/pope#XOR_Node> .
<http://w3id.org/abdn/policy/pope#Time> <http://www.w3.org/2000/01/rdf-schema#label> "Time"@en .
<http://w3id.org/abdn/policy/pope#Time> <http://www.w3.org/2000/01/rdf-schema#comment> "A role describing that the associated prov:Entity denoted an activity parameter containing some information about time used in some data processing activity."@en .
<http://w3id.org/abdn/policy/pope#Time> <http://www.w3.org/1999/02/22-rdf-syntax-ns#type> <http://w3id.org/abdn/policy/pope#Parameter> .
<http://w3id.org/abdn/policy/pope#Time> <http://www.w3.org/1999/02/22-rdf-syntax-ns#type> <http://www.w3.org/2002/07/owl#NamedIndividual> .
<http://w3id.org/abdn/policy/pope#Regex> <http://www.w3.org/2000/01/rdf-schema#comment> "Regex"@en .
<http://w3id.org/abdn/policy/pope#Regex> <http://www.w3.org/2000/01/rdf-schema#comment> "A role describing that the associated prov:Entity denoted an activity parameter containing some information about a regular expression used in some data processing activity."@en .
<http://w3id.org/abdn/policy/pope#Regex> <http://www.w3.org/1999/02/22-rdf-syntax-ns#type> <http://w3id.org/abdn/policy/pope#Parameter> .
<http://w3id.org/abdn/policy/pope#Regex> <http://www.w3.org/1999/02/22-rdf-syntax-ns#type> <http://www.w3.org/2002/07/owl#NamedIndividual> .
<http://w3id.org/abdn/policy/pope#Precondition> <http://www.w3.org/2000/01/rdf-schema#label> "Precondition"@en .
<http://w3id.org/abdn/policy/pope#Precondition> <http://www.w3.org/2000/01/rdf-schema#comment> "A kind of role describing that the associated prov:Entity denoted a poscondition constraint used by some activity describing a state of the world that entities conformed to before this activity ended. For example, a precondition can be described with a parameter denoting a threshold for the  maximum number of data items that can be processed by an activity."@en .
<http://w3id.org/abdn/policy/pope#Precondition> <http://www.w3.org/1999/02/22-rdf-syntax-ns#type> <http://w3id.org/abdn/policy/pope#Constraint> .
<http://w3id.org/abdn/policy/pope#Precondition> <http://www.w3.org/1999/02/22-rdf-syntax-ns#type> <http://www.w3.org/2002/07/owl#NamedIndividual> .
<http://w3id.org/abdn/policy/pope#DataFiltering> <http://www.w3.org/2000/01/rdf-schema#label> "Data Filtering"@en .
<http://w3id.org/abdn/policy/pope#DataFiltering> <http://www.w3.org/2000/01/rdf-schema#comment> "Filtering of data based on some parameters."@en .
<http://w3id.org/abdn/policy/pope#DataFiltering> <http://www.w3.org/1999/02/22-rdf-syntax-ns#type> <http://w3id.org/abdn/policy/pope#DataPreprocessing> .
<http://w3id.org/abdn/policy/pope#DataFiltering> <http://www.w3.org/1999/02/22-rdf-syntax-ns#type> <http://w3id.org/abdn/policy/pope#ActivityPlan> .
<http://w3id.org/abdn/policy/pope#DataFiltering> <http://www.w3.org/1999/02/22-rdf-syntax-ns#type> <http://www.w3.org/2002/07/owl#NamedIndividual> .
<http://w3id.org/abdn/policy/pope#matches> <http://www.w3.org/2000/01/rdf-schema#label> "matches"@en .
<http://w3id.org/abdn/policy/pope#matches> <http://www.w3.org/2000/01/rdf-schema#comment> "A matches B denotes that the expression described by the instance A can be matched on some value described by the instance B. For example, if A describes a regular expression, it can be matched on a piece of text described by B."@en .
<http://w3id.org/abdn/policy/pope#matches> <http://www.w3.org/2000/01/rdf-schema#subPropertyOf> <http://www.w3.org/2004/02/skos/core#related> .
<http://w3id.org/abdn/policy/pope#matches> <http://www.w3.org/1999/02/22-rdf-syntax-ns#type> <http://www.w3.org/2002/07/owl#ObjectProperty> .
<http://w3id.org/abdn/policy/pope#MultiLayerPerceptronNeuralNetworksSentimentAnalysis> <http://www.w3.org/2000/01/rdf-schema#label> "Multi-Layer Perceptron Neural Networks Sentiment Analysis"@en .
<http://w3id.org/abdn/policy/pope#MultiLayerPerceptronNeuralNetworksSentimentAnalysis> <http://www.w3.org/2000/01/rdf-schema#comment> "A sentiment analysis utilising the Multi-Layer Perceptron Neural Networks algorithm."@en .
<http://w3id.org/abdn/policy/pope#MultiLayerPerceptronNeuralNetworksSentimentAnalysis> <http://www.w3.org/1999/02/22-rdf-syntax-ns#type> <http://w3id.org/abdn/policy/pope#SentimentAnalysis> .
<http://w3id.org/abdn/policy/pope#MultiLayerPerceptronNeuralNetworksSentimentAnalysis> <http://www.w3.org/1999/02/22-rdf-syntax-ns#type> <http://w3id.org/abdn/policy/pope#DataAnalysis> .
<http://w3id.org/abdn/policy/pope#MultiLayerPerceptronNeuralNetworksSentimentAnalysis> <http://www.w3.org/1999/02/22-rdf-syntax-ns#type> <http://w3id.org/abdn/policy/pope#ActivityPlan> .
<http://w3id.org/abdn/policy/pope#MultiLayerPerceptronNeuralNetworksSentimentAnalysis> <http://www.w3.org/1999/02/22-rdf-syntax-ns#type> <http://www.w3.org/2002/07/owl#NamedIndividual> .
<http://w3id.org/abdn/policy/pope#WordFrequencyCount> <http://www.w3.org/2000/01/rdf-schema#label> "Word Frequency Count"@en .
<http://w3id.org/abdn/policy/pope#WordFrequencyCount> <http://www.w3.org/2000/01/rdf-schema#comment> "Analysis of single word frequency in a piece of text. Can be restricted by parameters specifying the number of top frequent words returned."@en .
<http://w3id.org/abdn/policy/pope#WordFrequencyCount> <http://www.w3.org/1999/02/22-rdf-syntax-ns#type> <http://w3id.org/abdn/policy/pope#DataAnalysis> .
<http://w3id.org/abdn/policy/pope#WordFrequencyCount> <http://www.w3.org/1999/02/22-rdf-syntax-ns#type> <http://w3id.org/abdn/policy/pope#ActivityPlan> .
<http://w3id.org/abdn/policy/pope#WordFrequencyCount> <http://www.w3.org/1999/02/22-rdf-syntax-ns#type> <http://www.w3.org/2002/07/owl#NamedIndividual> .
<http://w3id.org/abdn/policy/pope#includes> <http://www.w3.org/2000/01/rdf-schema#label> "includes"@en .
<http://w3id.org/abdn/policy/pope#includes> <http://www.w3.org/2000/01/rdf-schema#comment> "A includes B denotes that the instance A describes a concept that includes B. For example, if A is describing an area covering the UK, B can describe the city of London."@en .
<http://w3id.org/abdn/policy/pope#includes> <http://www.w3.org/2000/01/rdf-schema#subPropertyOf> <http://www.w3.org/2004/02/skos/core#related> .
<http://w3id.org/abdn/policy/pope#includes> <http://www.w3.org/1999/02/22-rdf-syntax-ns#type> <http://www.w3.org/2002/07/owl#ObjectProperty> .
<http://w3id.org/abdn/policy/pope#lhs> <http://www.w3.org/2000/01/rdf-schema#label> "lhs"@en .
<http://w3id.org/abdn/policy/pope#lhs> <http://www.w3.org/2000/01/rdf-schema#comment> "A property linking a parent node of a binary tree to its left hand side child."@en .
<http://w3id.org/abdn/policy/pope#lhs> <http://www.w3.org/2000/01/rdf-schema#range> _:A16aa612cX3aX1625a2637d3X3aXX2dX7ff8 .
<http://w3id.org/abdn/policy/pope#lhs> <http://www.w3.org/2000/01/rdf-schema#domain> _:A16aa612cX3aX1625a2637d3X3aXX2dX7ffc .
<http://w3id.org/abdn/policy/pope#lhs> <http://www.w3.org/1999/02/22-rdf-syntax-ns#type> <http://www.w3.org/2002/07/owl#FunctionalProperty> .
<http://w3id.org/abdn/policy/pope#lhs> <http://www.w3.org/2000/01/rdf-schema#subPropertyOf> <http://www.w3.org/2004/02/skos/core#related> .
<http://w3id.org/abdn/policy/pope#lhs> <http://www.w3.org/1999/02/22-rdf-syntax-ns#type> <http://www.w3.org/2002/07/owl#ObjectProperty> .
<http://w3id.org/abdn/policy/pope#DataRemoval> <http://www.w3.org/2000/01/rdf-schema#label> "Data Removal"@en .
<http://w3id.org/abdn/policy/pope#DataRemoval> <http://www.w3.org/2000/01/rdf-schema#comment> "Removal of data based on some parameters."@en .
<http://w3id.org/abdn/policy/pope#DataRemoval> <http://www.w3.org/1999/02/22-rdf-syntax-ns#type> <http://w3id.org/abdn/policy/pope#DataPreprocessing> .
<http://w3id.org/abdn/policy/pope#DataRemoval> <http://www.w3.org/1999/02/22-rdf-syntax-ns#type> <http://w3id.org/abdn/policy/pope#ActivityPlan> .
<http://w3id.org/abdn/policy/pope#DataRemoval> <http://www.w3.org/1999/02/22-rdf-syntax-ns#type> <http://www.w3.org/2002/07/owl#NamedIndividual> .
<http://w3id.org/abdn/policy/pope> <http://www.w3.org/2002/07/owl#imports> <http://www.w3.org/ns/prov-o-20130430> .
<http://w3id.org/abdn/policy/pope> <http://www.w3.org/2002/07/owl#imports> <http://www.w3.org/2004/02/skos/core> .
<http://w3id.org/abdn/policy/pope> <http://purl.org/dc/terms/creator> "Milan Markovic"^^<http://www.w3.org/2001/XMLSchema#string> .
<http://w3id.org/abdn/policy/pope> <http://purl.org/dc/terms/creator> "David Corsar"^^<http://www.w3.org/2001/XMLSchema#string> .
<http://w3id.org/abdn/policy/pope> <http://purl.org/dc/terms/license> "https://creativecommons.org/licenses/by/4.0/"^^<http://www.w3.org/2001/XMLSchema#string> .
<http://w3id.org/abdn/policy/pope> <http://www.w3.org/2000/01/rdf-schema#label> "PoPE Version 1.0"^^<http://www.w3.org/2001/XMLSchema#string> .
<http://w3id.org/abdn/policy/pope> <http://purl.org/dc/terms/description> "The PoPE Provenance Vocabulary defines a set of concepts and terms (the vocabulary)  for describing the use of social media data as evidence in policy-making."^^<http://www.w3.org/2001/XMLSchema#string> .
<http://w3id.org/abdn/policy/pope> <http://purl.org/dc/terms/creator> "Chenghua Lin"^^<http://www.w3.org/2001/XMLSchema#string> .
<http://w3id.org/abdn/policy/pope> <http://www.w3.org/2002/07/owl#versionInfo> "1.0"^^<http://www.w3.org/2001/XMLSchema#string> .
<http://w3id.org/abdn/policy/pope> <http://purl.org/dc/terms/creator> "Peter Edwards"^^<http://www.w3.org/2001/XMLSchema#string> .
<http://w3id.org/abdn/policy/pope> <http://www.w3.org/1999/02/22-rdf-syntax-ns#type> <http://www.w3.org/2002/07/owl#Ontology> .
_:A16aa612cX3aX1625a2637d3X3aXX2dX7ff7 <http://www.w3.org/1999/02/22-rdf-syntax-ns#rest> _:A16aa612cX3aX1625a2637d3X3aXX2dX7ff6 .
_:A16aa612cX3aX1625a2637d3X3aXX2dX7ff7 <http://www.w3.org/1999/02/22-rdf-syntax-ns#first> <http://w3id.org/abdn/policy/pope#AND_Node> .
<http://w3id.org/abdn/policy/pope#PopeSkosSchema> <http://www.w3.org/2000/01/rdf-schema#label> "PoPE Skos Schema"@en .
<http://w3id.org/abdn/policy/pope#PopeSkosSchema> <http://www.w3.org/2000/01/rdf-schema#comment> "PoPE skos schemea. Skos concepts defined using PoPE should be linked to this schema via skos:inSchema."@en .
<http://w3id.org/abdn/policy/pope#PopeSkosSchema> <http://www.w3.org/1999/02/22-rdf-syntax-ns#type> <http://www.w3.org/2004/02/skos/core#ConceptScheme> .
<http://w3id.org/abdn/policy/pope#PopeSkosSchema> <http://www.w3.org/1999/02/22-rdf-syntax-ns#type> <http://www.w3.org/2002/07/owl#NamedIndividual> .
<http://w3id.org/abdn/policy/pope#TextToUpperCase> <http://www.w3.org/2000/01/rdf-schema#label> "Text To Upper Case"@en .
<http://w3id.org/abdn/policy/pope#TextToUpperCase> <http://www.w3.org/2000/01/rdf-schema#comment> "Conversion of text to uppercase."@en .
<http://w3id.org/abdn/policy/pope#TextToUpperCase> <http://www.w3.org/1999/02/22-rdf-syntax-ns#type> <http://w3id.org/abdn/policy/pope#DataPreprocessing> .
<http://w3id.org/abdn/policy/pope#TextToUpperCase> <http://www.w3.org/1999/02/22-rdf-syntax-ns#type> <http://w3id.org/abdn/policy/pope#ActivityPlan> .
<http://w3id.org/abdn/policy/pope#TextToUpperCase> <http://www.w3.org/1999/02/22-rdf-syntax-ns#type> <http://www.w3.org/2002/07/owl#NamedIndividual> .
_:A16aa612cX3aX1625a2637d3X3aXX2dX7ff1 <http://www.w3.org/1999/02/22-rdf-syntax-ns#rest> _:A16aa612cX3aX1625a2637d3X3aXX2dX7ff0 .
_:A16aa612cX3aX1625a2637d3X3aXX2dX7ff1 <http://www.w3.org/1999/02/22-rdf-syntax-ns#first> <http://w3id.org/abdn/policy/pope#OR_Node> .
_:A16aa612cX3aX1625a2637d3X3aXX2dX7fea <http://www.w3.org/2000/01/rdf-schema#label> "Filtering Process"@en .
_:A16aa612cX3aX1625a2637d3X3aXX2dX7fea <http://www.w3.org/2000/01/rdf-schema#comment> "A kind of activity plan describing some data filtering process. The kind of filtering action is further described by prov:Entities used by the activity and described using pope:Parameter role, and associated PoPE subproperties of skos:related such as pope:includedIn, pope:subsumes, etc.   For example, and entity with the role pope:Keyword linked to the entities generated by the filtering activity via pope:includedIn denotes that the generated entities contain a specific keyword (subject to further constriants imposed on the parameters described using pope:Constraint)."@en .
_:A16aa612cX3aX1625a2637d3X3aXX2dX7fea <http://www.w3.org/2002/07/owl#annotatedTarget> <http://w3id.org/abdn/policy/pope#DataPreprocessing> .
_:A16aa612cX3aX1625a2637d3X3aXX2dX7fea <http://www.w3.org/2002/07/owl#annotatedProperty> <http://www.w3.org/1999/02/22-rdf-syntax-ns#type> .
_:A16aa612cX3aX1625a2637d3X3aXX2dX7fea <http://www.w3.org/2002/07/owl#annotatedSource> <http://w3id.org/abdn/policy/pope#DataFiltering> .
_:A16aa612cX3aX1625a2637d3X3aXX2dX7fea <http://www.w3.org/1999/02/22-rdf-syntax-ns#type> <http://www.w3.org/2002/07/owl#Axiom> .
<http://w3id.org/abdn/policy/pope#includedIn> <http://www.w3.org/2000/01/rdf-schema#label> "includedIn"@en .
<http://w3id.org/abdn/policy/pope#includedIn> <http://www.w3.org/2000/01/rdf-schema#comment> "A includedIn B denotes that the instance A describes a part of instance B. For example, if B is a dataset item, A can represent a portion of that item, for example, a body of a post contianed within B."@en .
<http://w3id.org/abdn/policy/pope#includedIn> <http://www.w3.org/2002/07/owl#inverseOf> <http://w3id.org/abdn/policy/pope#includes> .
<http://w3id.org/abdn/policy/pope#includedIn> <http://www.w3.org/2000/01/rdf-schema#subPropertyOf> <http://www.w3.org/2004/02/skos/core#related> .
<http://w3id.org/abdn/policy/pope#includedIn> <http://www.w3.org/1999/02/22-rdf-syntax-ns#type> <http://www.w3.org/2002/07/owl#ObjectProperty> .
_:A16aa612cX3aX1625a2637d3X3aXX2dX7fe9 <http://www.w3.org/2000/01/rdf-schema#label> "Data Removal"@en .
_:A16aa612cX3aX1625a2637d3X3aXX2dX7fe9 <http://www.w3.org/2000/01/rdf-schema#comment> "A kind of activity plan describing some data removal process (e.g. a stop word removal). The kind of action is further described by prov:Entities used by the activity and described using pope:Parameter role, and associated PoPE subproperties of skos:related such as pope:includedIn, pope:subsumes, etc.  For example, and entity with role pope:Keyword linked to the entities generated by the filtering activity via pope:notIncludedIn denotes that the generated entities do not contain a specific keyword (subject to further constriants imposed on the parameters described using pope:Constraint)."@en .
_:A16aa612cX3aX1625a2637d3X3aXX2dX7fe9 <http://www.w3.org/2002/07/owl#annotatedTarget> <http://w3id.org/abdn/policy/pope#DataPreprocessing> .
_:A16aa612cX3aX1625a2637d3X3aXX2dX7fe9 <http://www.w3.org/2002/07/owl#annotatedProperty> <http://www.w3.org/1999/02/22-rdf-syntax-ns#type> .
_:A16aa612cX3aX1625a2637d3X3aXX2dX7fe9 <http://www.w3.org/2002/07/owl#annotatedSource> <http://w3id.org/abdn/policy/pope#DataRemoval> .
_:A16aa612cX3aX1625a2637d3X3aXX2dX7fe9 <http://www.w3.org/1999/02/22-rdf-syntax-ns#type> <http://www.w3.org/2002/07/owl#Axiom> .
<http://w3id.org/abdn/policy/pope#isEqualTo> <http://www.w3.org/2000/01/rdf-schema#label> "isEqualTo"@en .
<http://w3id.org/abdn/policy/pope#isEqualTo> <http://www.w3.org/2000/01/rdf-schema#comment> "A isEqualTo B denotes that the value represented by instance A is equal to the value represented by instance B, however, A and B are not the same. For exampel, a red glass of water can be equal to a blue glass of water of the same size."@en .
<http://w3id.org/abdn/policy/pope#isEqualTo> <http://www.w3.org/1999/02/22-rdf-syntax-ns#type> <http://www.w3.org/2002/07/owl#SymmetricProperty> .
<http://w3id.org/abdn/policy/pope#isEqualTo> <http://www.w3.org/2000/01/rdf-schema#subPropertyOf> <http://www.w3.org/2004/02/skos/core#related> .
<http://w3id.org/abdn/policy/pope#isEqualTo> <http://www.w3.org/1999/02/22-rdf-syntax-ns#type> <http://www.w3.org/2002/07/owl#ObjectProperty> .
<http://w3id.org/abdn/policy/pope#GroupTag> <http://www.w3.org/2000/01/rdf-schema#label> "Group Tag"@en .
<http://w3id.org/abdn/policy/pope#GroupTag> <http://www.w3.org/2000/01/rdf-schema#comment> "A role describing that the associated prov:Entity denoted an activity parameter containing some information about a group tag (e.g. to group multiple search activities) used in some data processing activity."@en .
<http://w3id.org/abdn/policy/pope#GroupTag> <http://www.w3.org/1999/02/22-rdf-syntax-ns#type> <http://w3id.org/abdn/policy/pope#Parameter> .
<http://w3id.org/abdn/policy/pope#GroupTag> <http://www.w3.org/1999/02/22-rdf-syntax-ns#type> <http://www.w3.org/2002/07/owl#NamedIndividual> .
<http://w3id.org/abdn/policy/pope#PostID> <http://www.w3.org/2000/01/rdf-schema#label> "Post ID"@en .
<http://w3id.org/abdn/policy/pope#PostID> <http://www.w3.org/2000/01/rdf-schema#comment> "A role describing that the associated prov:Entity denoted an activity parameter containing some information about an ID of a social media post used in some data processing activity."@en .
<http://w3id.org/abdn/policy/pope#PostID> <http://www.w3.org/1999/02/22-rdf-syntax-ns#type> <http://w3id.org/abdn/policy/pope#Parameter> .
<http://w3id.org/abdn/policy/pope#PostID> <http://www.w3.org/1999/02/22-rdf-syntax-ns#type> <http://www.w3.org/2002/07/owl#NamedIndividual> .
<http://w3id.org/abdn/policy/pope#moreThan> <http://www.w3.org/2000/01/rdf-schema#label> "moreThan"@en .
<http://w3id.org/abdn/policy/pope#moreThan> <http://www.w3.org/2000/01/rdf-schema#comment> "A moreThan B denotes that the quantity represented by instance A is greater than the quantity represented by instance B."@en .
<http://w3id.org/abdn/policy/pope#moreThan> <http://www.w3.org/2000/01/rdf-schema#subPropertyOf> <http://www.w3.org/2004/02/skos/core#related> .
<http://w3id.org/abdn/policy/pope#moreThan> <http://www.w3.org/1999/02/22-rdf-syntax-ns#type> <http://www.w3.org/2002/07/owl#ObjectProperty> .
<http://w3id.org/abdn/policy/pope#parameter> <http://www.w3.org/2000/01/rdf-schema#label> "parameter"@en .
<http://w3id.org/abdn/policy/pope#parameter> <http://www.w3.org/2000/01/rdf-schema#comment> "A property for linking pope:LeafNode to a prov:Entity typically associated with a role of pope:Parameter."@en .
<http://w3id.org/abdn/policy/pope#parameter> <http://www.w3.org/2000/01/rdf-schema#range> <http://www.w3.org/ns/prov#Entity> .
<http://w3id.org/abdn/policy/pope#parameter> <http://www.w3.org/2000/01/rdf-schema#domain> <http://w3id.org/abdn/policy/pope#LeafNode> .
<http://w3id.org/abdn/policy/pope#parameter> <http://www.w3.org/2000/01/rdf-schema#subPropertyOf> <http://www.w3.org/2004/02/skos/core#related> .
<http://w3id.org/abdn/policy/pope#parameter> <http://www.w3.org/1999/02/22-rdf-syntax-ns#type> <http://www.w3.org/2002/07/owl#ObjectProperty> .
<http://w3id.org/abdn/policy/pope#StatisticalMeasure> <http://www.w3.org/2000/01/rdf-schema#label> "Statistical Measure"@en .
<http://w3id.org/abdn/policy/pope#StatisticalMeasure> <http://www.w3.org/2000/01/rdf-schema#comment> "A role describing that the associated prov:Entity denoted an activity parameter containing some information about a statistical measure (e.g.  dataset size) used in some data processing activity."@en .
<http://w3id.org/abdn/policy/pope#StatisticalMeasure> <http://www.w3.org/1999/02/22-rdf-syntax-ns#type> <http://w3id.org/abdn/policy/pope#Parameter> .
<http://w3id.org/abdn/policy/pope#StatisticalMeasure> <http://www.w3.org/1999/02/22-rdf-syntax-ns#type> <http://www.w3.org/2002/07/owl#NamedIndividual> .
_:A16aa612cX3aX1625a2637d3X3aXX2dX7ff6 <http://www.w3.org/1999/02/22-rdf-syntax-ns#rest> _:A16aa612cX3aX1625a2637d3X3aXX2dX7ff5 .
_:A16aa612cX3aX1625a2637d3X3aXX2dX7ff6 <http://www.w3.org/1999/02/22-rdf-syntax-ns#first> <http://w3id.org/abdn/policy/pope#LeafNode> .
_:A16aa612cX3aX1625a2637d3X3aXX2dX7fef <http://www.w3.org/2002/07/owl#unionOf> _:A16aa612cX3aX1625a2637d3X3aXX2dX7fee .
_:A16aa612cX3aX1625a2637d3X3aXX2dX7fef <http://www.w3.org/1999/02/22-rdf-syntax-ns#type> <http://www.w3.org/2002/07/owl#Class> .
_:A16aa612cX3aX1625a2637d3X3aXX2dX7ff0 <http://www.w3.org/1999/02/22-rdf-syntax-ns#rest> <http://www.w3.org/1999/02/22-rdf-syntax-ns#nil> .
_:A16aa612cX3aX1625a2637d3X3aXX2dX7ff0 <http://www.w3.org/1999/02/22-rdf-syntax-ns#first> <http://w3id.org/abdn/policy/pope#XOR_Node> .
<http://w3id.org/abdn/policy/pope#TopicExtractionDataSet> <http://www.w3.org/2000/01/rdf-schema#label> "Topic Extraction Dataset"@en .
<http://w3id.org/abdn/policy/pope#TopicExtractionDataSet> <http://www.w3.org/2000/01/rdf-schema#comment> "A kind of role describing that the associated prov:Entity denoted a prov:Collection representing topic extraction results collection."@en .
<http://w3id.org/abdn/policy/pope#TopicExtractionDataSet> <http://www.w3.org/1999/02/22-rdf-syntax-ns#type> <http://w3id.org/abdn/policy/pope#DataSet> .
<http://w3id.org/abdn/policy/pope#TopicExtractionDataSet> <http://www.w3.org/1999/02/22-rdf-syntax-ns#type> <http://www.w3.org/2002/07/owl#NamedIndividual> .
_:A16aa612cX3aX1625a2637d3X3aXX2dX7ffc <http://www.w3.org/2002/07/owl#unionOf> _:A16aa612cX3aX1625a2637d3X3aXX2dX7ffb .
_:A16aa612cX3aX1625a2637d3X3aXX2dX7ffc <http://www.w3.org/1999/02/22-rdf-syntax-ns#type> <http://www.w3.org/2002/07/owl#Class> .
<http://w3id.org/abdn/policy/pope#ApiEndpoint> <http://www.w3.org/2000/01/rdf-schema#label> "API Endpoint"@en .
<http://w3id.org/abdn/policy/pope#ApiEndpoint> <http://www.w3.org/2000/01/rdf-schema#comment> "A role describing that the associated prov:Entity denoted an activity parameter containing some information about an API reference endpoint used in some data processing activity."@en .
<http://w3id.org/abdn/policy/pope#ApiEndpoint> <http://www.w3.org/1999/02/22-rdf-syntax-ns#type> <http://w3id.org/abdn/policy/pope#Parameter> .
<http://w3id.org/abdn/policy/pope#ApiEndpoint> <http://www.w3.org/1999/02/22-rdf-syntax-ns#type> <http://www.w3.org/2002/07/owl#NamedIndividual> .
_:A16aa612cX3aX1625a2637d3X3aXX2dX7fe8 <http://www.w3.org/2000/01/rdf-schema#label> "Postcondition"@en .
_:A16aa612cX3aX1625a2637d3X3aXX2dX7fe8 <http://www.w3.org/2000/01/rdf-schema#comment> "An activity postcondition describes a state of the world that generated entities conformed to. The state is described as logical groupings of one or more pope:Parameter use dby the activity and semantically linked with subproperties of skos:related to some characterists of generated datasets or dataset items."@en .
_:A16aa612cX3aX1625a2637d3X3aXX2dX7fe8 <http://www.w3.org/2002/07/owl#annotatedTarget> <http://w3id.org/abdn/policy/pope#Constraint> .
_:A16aa612cX3aX1625a2637d3X3aXX2dX7fe8 <http://www.w3.org/2002/07/owl#annotatedProperty> <http://www.w3.org/1999/02/22-rdf-syntax-ns#type> .
_:A16aa612cX3aX1625a2637d3X3aXX2dX7fe8 <http://www.w3.org/2002/07/owl#annotatedSource> <http://w3id.org/abdn/policy/pope#Postcondition> .
_:A16aa612cX3aX1625a2637d3X3aXX2dX7fe8 <http://www.w3.org/1999/02/22-rdf-syntax-ns#type> <http://www.w3.org/2002/07/owl#Axiom> .
<http://w3id.org/abdn/policy/pope#moreThanOrEqualTo> <http://www.w3.org/2000/01/rdf-schema#label> "moreThanOrEqualTo"@en .
<http://w3id.org/abdn/policy/pope#moreThanOrEqualTo> <http://www.w3.org/2000/01/rdf-schema#comment> "A moreThanOrEqualTo B denotes that the quantity represented by instance A is greater or equal to the quantity represented by instance B."@en .
<http://w3id.org/abdn/policy/pope#moreThanOrEqualTo> <http://www.w3.org/2000/01/rdf-schema#subPropertyOf> <http://www.w3.org/2004/02/skos/core#related> .
<http://w3id.org/abdn/policy/pope#moreThanOrEqualTo> <http://www.w3.org/1999/02/22-rdf-syntax-ns#type> <http://www.w3.org/2002/07/owl#ObjectProperty> .
_:A16aa612cX3aX1625a2637d3X3aXX2dX7ff5 <http://www.w3.org/1999/02/22-rdf-syntax-ns#rest> _:A16aa612cX3aX1625a2637d3X3aXX2dX7ff4 .
_:A16aa612cX3aX1625a2637d3X3aXX2dX7ff5 <http://www.w3.org/1999/02/22-rdf-syntax-ns#first> <http://w3id.org/abdn/policy/pope#OR_Node> .
_:A16aa612cX3aX1625a2637d3X3aXX2dX7fee <http://www.w3.org/1999/02/22-rdf-syntax-ns#rest> _:A16aa612cX3aX1625a2637d3X3aXX2dX7fed .
_:A16aa612cX3aX1625a2637d3X3aXX2dX7fee <http://www.w3.org/1999/02/22-rdf-syntax-ns#first> <http://w3id.org/abdn/policy/pope#AND_Node> .
<http://w3id.org/abdn/policy/pope#lessThanOrEqualTo> <http://www.w3.org/2000/01/rdf-schema#label> "lessThanOrEqualTo"@en .
<http://w3id.org/abdn/policy/pope#lessThanOrEqualTo> <http://www.w3.org/2000/01/rdf-schema#comment> "A lessThanOrEqualTo B denotes that the quantity represented by instance A is lower or equal to the quantity represented by instance B."@en .
<http://w3id.org/abdn/policy/pope#lessThanOrEqualTo> <http://www.w3.org/2002/07/owl#inverseOf> <http://w3id.org/abdn/policy/pope#moreThanOrEqualTo> .
<http://w3id.org/abdn/policy/pope#lessThanOrEqualTo> <http://www.w3.org/2000/01/rdf-schema#subPropertyOf> <http://www.w3.org/2004/02/skos/core#related> .
<http://w3id.org/abdn/policy/pope#lessThanOrEqualTo> <http://www.w3.org/1999/02/22-rdf-syntax-ns#type> <http://www.w3.org/2002/07/owl#ObjectProperty> .
<http://w3id.org/abdn/policy/pope#DataPreprocessing> <http://www.w3.org/2000/01/rdf-schema#label> "Data Preprocessing"@en .
<http://w3id.org/abdn/policy/pope#DataPreprocessing> <http://www.w3.org/2000/01/rdf-schema#comment> "A kind of activity plan describing the process of data preprocessing (e.g. stop words removal, filtering, text case transformation, etc.)"@en .
<http://w3id.org/abdn/policy/pope#DataPreprocessing> <http://www.w3.org/2000/01/rdf-schema#subClassOf> <http://w3id.org/abdn/policy/pope#ActivityPlan> .
<http://w3id.org/abdn/policy/pope#DataPreprocessing> <http://www.w3.org/1999/02/22-rdf-syntax-ns#type> <http://www.w3.org/2002/07/owl#Class> .
<http://w3id.org/abdn/policy/pope#Constraint> <http://www.w3.org/2000/01/rdf-schema#label> "Constraint"@en .
<http://w3id.org/abdn/policy/pope#Constraint> <http://www.w3.org/2000/01/rdf-schema#comment> "A kind of role describing that the associated prov:Entity denoted some condition/state of the world further described by enties associated with role pope:Parameter. It can be further described with pope:describedAs property linking to a  skos:Concept. For example, a binary tree using pope:AND_Node, pope:OR_Node, pope:XOR_Node and pope:LeafNode can be used to represent logical groupings of one or more of activity parameters."@en .
<http://w3id.org/abdn/policy/pope#Constraint> <http://www.w3.org/2000/01/rdf-schema#subClassOf> <http://www.w3.org/ns/prov#Role> .
<http://w3id.org/abdn/policy/pope#Constraint> <http://www.w3.org/1999/02/22-rdf-syntax-ns#type> <http://www.w3.org/2002/07/owl#Class> .
<http://w3id.org/abdn/policy/pope#Keyword> <http://www.w3.org/2000/01/rdf-schema#label> "Keyword"@en .
<http://w3id.org/abdn/policy/pope#Keyword> <http://www.w3.org/2000/01/rdf-schema#comment> "A role describing that the associated prov:Entity denoted an activity parameter containing some information about a keyword used in some data processing activity."@en .
<http://w3id.org/abdn/policy/pope#Keyword> <http://www.w3.org/1999/02/22-rdf-syntax-ns#type> <http://w3id.org/abdn/policy/pope#Parameter> .
<http://w3id.org/abdn/policy/pope#Keyword> <http://www.w3.org/1999/02/22-rdf-syntax-ns#type> <http://www.w3.org/2002/07/owl#NamedIndividual> .
<http://w3id.org/abdn/policy/pope#DataAnalysis> <http://www.w3.org/2000/01/rdf-schema#label> "Data Analysis"@en .
<http://w3id.org/abdn/policy/pope#DataAnalysis> <http://www.w3.org/2000/01/rdf-schema#comment> "A kind of  activity plan describing the process of data analysis (e.g. sentiment analysis, word frequency count, etc.)"@en .
<http://w3id.org/abdn/policy/pope#DataAnalysis> <http://www.w3.org/2000/01/rdf-schema#subClassOf> <http://w3id.org/abdn/policy/pope#ActivityPlan> .
<http://w3id.org/abdn/policy/pope#DataAnalysis> <http://www.w3.org/1999/02/22-rdf-syntax-ns#type> <http://www.w3.org/2002/07/owl#Class> .
_:A16aa612cX3aX1625a2637d3X3aXX2dX7ffb <http://www.w3.org/1999/02/22-rdf-syntax-ns#rest> _:A16aa612cX3aX1625a2637d3X3aXX2dX7ffa .
_:A16aa612cX3aX1625a2637d3X3aXX2dX7ffb <http://www.w3.org/1999/02/22-rdf-syntax-ns#first> <http://w3id.org/abdn/policy/pope#AND_Node> .
_:A16aa612cX3aX1625a2637d3X3aXX2dX7fe7 <http://www.w3.org/2000/01/rdf-schema#label> "Precondition"@en .
_:A16aa612cX3aX1625a2637d3X3aXX2dX7fe7 <http://www.w3.org/2000/01/rdf-schema#comment> "An activity precondition describes a state of the world that used entities conformed to. The state is described as logical groupings of one or more pope:Parameter used by the activity and semantically linked with subproperties of skos:related to some characterists of used datasets or dataset items."@en .
_:A16aa612cX3aX1625a2637d3X3aXX2dX7fe7 <http://www.w3.org/2002/07/owl#annotatedTarget> <http://w3id.org/abdn/policy/pope#Constraint> .
_:A16aa612cX3aX1625a2637d3X3aXX2dX7fe7 <http://www.w3.org/2002/07/owl#annotatedProperty> <http://www.w3.org/1999/02/22-rdf-syntax-ns#type> .
_:A16aa612cX3aX1625a2637d3X3aXX2dX7fe7 <http://www.w3.org/2002/07/owl#annotatedSource> <http://w3id.org/abdn/policy/pope#Precondition> .
_:A16aa612cX3aX1625a2637d3X3aXX2dX7fe7 <http://www.w3.org/1999/02/22-rdf-syntax-ns#type> <http://www.w3.org/2002/07/owl#Axiom> .
<http://w3id.org/abdn/policy/pope#ActivityPlan> <http://www.w3.org/2000/01/rdf-schema#label> "Activity Plan"@en .
<http://w3id.org/abdn/policy/pope#ActivityPlan> <http://www.w3.org/2000/01/rdf-schema#comment> "ActivityPlans describe the type of plan followed by an agent to guide their activity in relation to, for example, collection of data, processing of data before analysis, or analysis of the data.  It is not the intent of ActivityPlan to provide a breakdown of the steps or actions that are involved in the plan; this type of information can, if desired, be represented with alternative plan representations."@en .
<http://w3id.org/abdn/policy/pope#ActivityPlan> <http://www.w3.org/2000/01/rdf-schema#subClassOf> <http://www.w3.org/ns/prov#Plan> .
<http://w3id.org/abdn/policy/pope#ActivityPlan> <http://www.w3.org/1999/02/22-rdf-syntax-ns#type> <http://www.w3.org/2002/07/owl#Class> .
<http://w3id.org/abdn/policy/pope#SentimentAnalysisDataSet> <http://www.w3.org/2000/01/rdf-schema#label> "Sentiment Analysis Dataset"@en .
<http://w3id.org/abdn/policy/pope#SentimentAnalysisDataSet> <http://www.w3.org/2000/01/rdf-schema#comment> "A kind of role describing that the associated prov:Entity denoted a prov:Collection representing  sentiment analysis results collection."@en .
<http://w3id.org/abdn/policy/pope#SentimentAnalysisDataSet> <http://www.w3.org/1999/02/22-rdf-syntax-ns#type> <http://w3id.org/abdn/policy/pope#DataSet> .
<http://w3id.org/abdn/policy/pope#SentimentAnalysisDataSet> <http://www.w3.org/1999/02/22-rdf-syntax-ns#type> <http://www.w3.org/2002/07/owl#NamedIndividual> .
<http://w3id.org/abdn/policy/pope#Postcondition> <http://www.w3.org/2000/01/rdf-schema#label> "Postcondition"@en .
<http://w3id.org/abdn/policy/pope#Postcondition> <http://www.w3.org/2000/01/rdf-schema#comment> "A kind of role describing that the associated prov:Entity denoted a poscondition constraint used by some activity describing a state of the world that entities generated this activity conformed to."@en .
<http://w3id.org/abdn/policy/pope#Postcondition> <http://www.w3.org/1999/02/22-rdf-syntax-ns#type> <http://w3id.org/abdn/policy/pope#Constraint> .
<http://w3id.org/abdn/policy/pope#Postcondition> <http://www.w3.org/1999/02/22-rdf-syntax-ns#type> <http://www.w3.org/2002/07/owl#NamedIndividual> .
<http://w3id.org/abdn/policy/pope#CollectionViaApi> <http://www.w3.org/2000/01/rdf-schema#label> "Collection via API"@en .
<http://w3id.org/abdn/policy/pope#CollectionViaApi> <http://www.w3.org/2000/01/rdf-schema#comment> "Collection of data retrieved via an API."@en .
<http://w3id.org/abdn/policy/pope#CollectionViaApi> <http://www.w3.org/1999/02/22-rdf-syntax-ns#type> <http://w3id.org/abdn/policy/pope#DataCollection> .
<http://w3id.org/abdn/policy/pope#CollectionViaApi> <http://www.w3.org/1999/02/22-rdf-syntax-ns#type> <http://w3id.org/abdn/policy/pope#ActivityPlan> .
<http://w3id.org/abdn/policy/pope#CollectionViaApi> <http://www.w3.org/1999/02/22-rdf-syntax-ns#type> <http://www.w3.org/2002/07/owl#NamedIndividual> .
<http://w3id.org/abdn/policy/pope#notIncludedIn> <http://www.w3.org/2000/01/rdf-schema#label> "notIncludedIn"@en .
<http://w3id.org/abdn/policy/pope#notIncludedIn> <http://www.w3.org/2000/01/rdf-schema#comment> "A notIncludedIn B denotes that the instance A does not describe any part of instance B. For example, if B represents a piece of text, A can represent a keyword that is not present in B."@en .
<http://w3id.org/abdn/policy/pope#notIncludedIn> <http://www.w3.org/2000/01/rdf-schema#subPropertyOf> <http://www.w3.org/2004/02/skos/core#related> .
<http://w3id.org/abdn/policy/pope#notIncludedIn> <http://www.w3.org/1999/02/22-rdf-syntax-ns#type> <http://www.w3.org/2002/07/owl#ObjectProperty> .
<http://w3id.org/abdn/policy/pope#TopicExtraction> <http://www.w3.org/2000/01/rdf-schema#label> "Topic Extraction"@en .
<http://w3id.org/abdn/policy/pope#TopicExtraction> <http://www.w3.org/2000/01/rdf-schema#comment> "A kind activity plan describing  analysis that utilise and algorithm for extracting topics from a corpus of documents."@en .
<http://w3id.org/abdn/policy/pope#TopicExtraction> <http://www.w3.org/2000/01/rdf-schema#subClassOf> <http://w3id.org/abdn/policy/pope#DataAnalysis> .
<http://w3id.org/abdn/policy/pope#TopicExtraction> <http://www.w3.org/1999/02/22-rdf-syntax-ns#type> <http://www.w3.org/2002/07/owl#Class> .
<http://w3id.org/abdn/policy/pope#TwitterDataset> <http://www.w3.org/2000/01/rdf-schema#label> "Twitter Dataset"@en .
<http://w3id.org/abdn/policy/pope#TwitterDataset> <http://www.w3.org/2000/01/rdf-schema#comment> "A kind of role describing that the associated prov:Entity denoted a prov:Collection representing a collection of posts from Twitter social media platform."@en .
<http://w3id.org/abdn/policy/pope#TwitterDataset> <http://www.w3.org/1999/02/22-rdf-syntax-ns#type> <http://w3id.org/abdn/policy/pope#DataSet> .
<http://w3id.org/abdn/policy/pope#TwitterDataset> <http://www.w3.org/1999/02/22-rdf-syntax-ns#type> <http://www.w3.org/2002/07/owl#NamedIndividual> .
_:A16aa612cX3aX1625a2637d3X3aXX2dX7ff4 <http://www.w3.org/1999/02/22-rdf-syntax-ns#rest> <http://www.w3.org/1999/02/22-rdf-syntax-ns#nil> .
_:A16aa612cX3aX1625a2637d3X3aXX2dX7ff4 <http://www.w3.org/1999/02/22-rdf-syntax-ns#first> <http://w3id.org/abdn/policy/pope#XOR_Node> .
<http://w3id.org/abdn/policy/pope#lessThan> <http://www.w3.org/2000/01/rdf-schema#label> "lessThan"@en .
<http://w3id.org/abdn/policy/pope#lessThan> <http://www.w3.org/2000/01/rdf-schema#comment> "A lessThan B denotes that the quantity represented by instance A is lower than the quantity represented by instance B."@en .
<http://w3id.org/abdn/policy/pope#lessThan> <http://www.w3.org/2002/07/owl#inverseOf> <http://w3id.org/abdn/policy/pope#moreThan> .
<http://w3id.org/abdn/policy/pope#lessThan> <http://www.w3.org/2000/01/rdf-schema#subPropertyOf> <http://www.w3.org/2004/02/skos/core#related> .
<http://w3id.org/abdn/policy/pope#lessThan> <http://www.w3.org/1999/02/22-rdf-syntax-ns#type> <http://www.w3.org/2002/07/owl#ObjectProperty> .
_:A16aa612cX3aX1625a2637d3X3aXX2dX7fed <http://www.w3.org/1999/02/22-rdf-syntax-ns#rest> _:A16aa612cX3aX1625a2637d3X3aXX2dX7fec .
_:A16aa612cX3aX1625a2637d3X3aXX2dX7fed <http://www.w3.org/1999/02/22-rdf-syntax-ns#first> <http://w3id.org/abdn/policy/pope#LeafNode> .
<http://w3id.org/abdn/policy/pope#OR_Node> <http://www.w3.org/2000/01/rdf-schema#label> "OR Node"@en .
<http://w3id.org/abdn/policy/pope#OR_Node> <http://www.w3.org/2000/01/rdf-schema#comment> "A concept describing an inner node of a binary tree structure. The node represents the logical operator OR  in a binary tree description of pope:Constraint. If A is an OR_Node and B and C are children of A then  test on conditions specified by B OR C equals true."@en .
<http://w3id.org/abdn/policy/pope#OR_Node> <http://www.w3.org/2002/07/owl#disjointWith> <http://w3id.org/abdn/policy/pope#XOR_Node> .
<http://w3id.org/abdn/policy/pope#OR_Node> <http://www.w3.org/2000/01/rdf-schema#subClassOf> <http://www.w3.org/2004/02/skos/core#Concept> .
<http://w3id.org/abdn/policy/pope#OR_Node> <http://www.w3.org/1999/02/22-rdf-syntax-ns#type> <http://www.w3.org/2002/07/owl#Class> .
<http://w3id.org/abdn/policy/pope#LDA_TopicExtraction> <http://www.w3.org/2000/01/rdf-schema#label> "Latent Dirichlet Allocation Topic Exctraction"@en .
<http://w3id.org/abdn/policy/pope#LDA_TopicExtraction> <http://www.w3.org/2000/01/rdf-schema#comment> "A topic extraction utilising the LDA algorithm."@en .
<http://w3id.org/abdn/policy/pope#LDA_TopicExtraction> <http://www.w3.org/1999/02/22-rdf-syntax-ns#type> <http://w3id.org/abdn/policy/pope#TopicExtraction> .
<http://w3id.org/abdn/policy/pope#LDA_TopicExtraction> <http://www.w3.org/1999/02/22-rdf-syntax-ns#type> <http://w3id.org/abdn/policy/pope#DataAnalysis> .
<http://w3id.org/abdn/policy/pope#LDA_TopicExtraction> <http://www.w3.org/1999/02/22-rdf-syntax-ns#type> <http://w3id.org/abdn/policy/pope#ActivityPlan> .
<http://w3id.org/abdn/policy/pope#LDA_TopicExtraction> <http://www.w3.org/1999/02/22-rdf-syntax-ns#type> <http://www.w3.org/2002/07/owl#NamedIndividual> .
<http://w3id.org/abdn/policy/pope#XOR_Node> <http://www.w3.org/2000/01/rdf-schema#label> "XOR Node"@en .
<http://w3id.org/abdn/policy/pope#XOR_Node> <http://www.w3.org/2000/01/rdf-schema#comment> "A concept describing an inner node of a binary tree structure. The node represents the logical operator XOR in a binary tree description of pope:Constraint. If A is an XOR_Node and B and C are children of A then test on conditions specified by B XOR C equals true."@en .
<http://w3id.org/abdn/policy/pope#XOR_Node> <http://www.w3.org/2000/01/rdf-schema#subClassOf> <http://www.w3.org/2004/02/skos/core#Concept> .
<http://w3id.org/abdn/policy/pope#XOR_Node> <http://www.w3.org/1999/02/22-rdf-syntax-ns#type> <http://www.w3.org/2002/07/owl#Class> .
<http://w3id.org/abdn/policy/pope#AND_Node> <http://www.w3.org/2000/01/rdf-schema#label> "AND Node"@en .
<http://w3id.org/abdn/policy/pope#AND_Node> <http://www.w3.org/2000/01/rdf-schema#comment> "A concept describing an inner node of a binary tree structure. The node represents the logical operator AND in a binary tree description of pope:Constraint. If A is an XOR_Node and B and C are children of A then test on conditions specified by B AND C equals true."@en .
<http://w3id.org/abdn/policy/pope#AND_Node> <http://www.w3.org/2002/07/owl#disjointWith> <http://w3id.org/abdn/policy/pope#XOR_Node> .
<http://w3id.org/abdn/policy/pope#AND_Node> <http://www.w3.org/2002/07/owl#disjointWith> <http://w3id.org/abdn/policy/pope#OR_Node> .
<http://w3id.org/abdn/policy/pope#AND_Node> <http://www.w3.org/2002/07/owl#disjointWith> <http://w3id.org/abdn/policy/pope#LeafNode> .
<http://w3id.org/abdn/policy/pope#AND_Node> <http://www.w3.org/2000/01/rdf-schema#subClassOf> <http://www.w3.org/2004/02/skos/core#Concept> .
<http://w3id.org/abdn/policy/pope#AND_Node> <http://www.w3.org/1999/02/22-rdf-syntax-ns#type> <http://www.w3.org/2002/07/owl#Class> .
<http://w3id.org/abdn/policy/pope#TextToLowerCase> <http://www.w3.org/2000/01/rdf-schema#label> "Text To Lower Case"@en .
<http://w3id.org/abdn/policy/pope#TextToLowerCase> <http://www.w3.org/2000/01/rdf-schema#comment> "Conversion of text to lowercase."@en .
<http://w3id.org/abdn/policy/pope#TextToLowerCase> <http://www.w3.org/1999/02/22-rdf-syntax-ns#type> <http://w3id.org/abdn/policy/pope#DataPreprocessing> .
<http://w3id.org/abdn/policy/pope#TextToLowerCase> <http://www.w3.org/1999/02/22-rdf-syntax-ns#type> <http://w3id.org/abdn/policy/pope#ActivityPlan> .
<http://w3id.org/abdn/policy/pope#TextToLowerCase> <http://www.w3.org/1999/02/22-rdf-syntax-ns#type> <http://www.w3.org/2002/07/owl#NamedIndividual> .
_:A16aa612cX3aX1625a2637d3X3aXX2dX7ffa <http://www.w3.org/1999/02/22-rdf-syntax-ns#rest> _:A16aa612cX3aX1625a2637d3X3aXX2dX7ff9 .
_:A16aa612cX3aX1625a2637d3X3aXX2dX7ffa <http://www.w3.org/1999/02/22-rdf-syntax-ns#first> <http://w3id.org/abdn/policy/pope#OR_Node> .
<http://w3id.org/abdn/policy/pope#Location> <http://www.w3.org/2000/01/rdf-schema#label> "Location"@en .
<http://w3id.org/abdn/policy/pope#Location> <http://www.w3.org/2000/01/rdf-schema#comment> "A role describing that the associated prov:Entity denoted an activity parameter containing some information about a location used in some data processing activity."@en .
<http://w3id.org/abdn/policy/pope#Location> <http://www.w3.org/1999/02/22-rdf-syntax-ns#type> <http://w3id.org/abdn/policy/pope#Parameter> .
<http://w3id.org/abdn/policy/pope#Location> <http://www.w3.org/1999/02/22-rdf-syntax-ns#type> <http://www.w3.org/2002/07/owl#NamedIndividual> .
<http://w3id.org/abdn/policy/pope#describedAs> <http://www.w3.org/2000/01/rdf-schema#subPropertyOf> <http://www.w3.org/2004/02/skos/core#narrower> .
<http://w3id.org/abdn/policy/pope#describedAs> <http://www.w3.org/1999/02/22-rdf-syntax-ns#type> <http://www.w3.org/2002/07/owl#ObjectProperty> .
_:A16aa612cX3aX1625a2637d3X3aXX2dX7fe6 <http://www.w3.org/2000/01/rdf-schema#label> "Text to lowercase"@en .
_:A16aa612cX3aX1625a2637d3X3aXX2dX7fe6 <http://www.w3.org/2000/01/rdf-schema#comment> "A kind of activity plan describing a process converting text to lowercase. This kind of action is further described by prov:Entities used by the activity and described using pope:Parameter role, and associated PoPE subproperties of skos:related such as pope:includedIn, pope:subsumes, etc.   For example, and entity with role pope:Regex representing uppercase letters linked to some characteristics of entities (data items) generated by the activity via pope:doesNotMatch denotes that the generated entities contain a text that does not contain any uppercase letters (subject to further constriants imposed on the parameters described using pope:Constraint)."@en .
_:A16aa612cX3aX1625a2637d3X3aXX2dX7fe6 <http://www.w3.org/2002/07/owl#annotatedTarget> <http://w3id.org/abdn/policy/pope#DataPreprocessing> .
_:A16aa612cX3aX1625a2637d3X3aXX2dX7fe6 <http://www.w3.org/2002/07/owl#annotatedProperty> <http://www.w3.org/1999/02/22-rdf-syntax-ns#type> .
_:A16aa612cX3aX1625a2637d3X3aXX2dX7fe6 <http://www.w3.org/2002/07/owl#annotatedSource> <http://w3id.org/abdn/policy/pope#TextToLowerCase> .
_:A16aa612cX3aX1625a2637d3X3aXX2dX7fe6 <http://www.w3.org/1999/02/22-rdf-syntax-ns#type> <http://www.w3.org/2002/07/owl#Axiom> .
